examples/pseudo_bool/cp_encoding/cp_to_ilp_linearScript.sml
@@ -7,6 +7,113 @@ Libs
 Ancestors
   pbc cp ilp cp_to_ilp
 
+Definition mk_lin_ge_def[simp]:
+  mk_lin_ge cXs Y = mk_lin_constraint_ge ((-1i,Y)::cXs) 0
+End
+
+Definition mk_lin_le_def[simp]:
+  mk_lin_le cXs Y = mk_lin_constraint_ge ((1i,Y)::(MAP (λ(c,X). (-c,X)) cXs)) 0
+End
+
+Definition mk_lin_gt_def[simp]:
+  mk_lin_gt cXs Y = mk_lin_constraint_ge ((-1i,Y)::cXs) 1
+End
+
+Definition mk_lin_lt_def[simp]:
+  mk_lin_lt cXs Y = mk_lin_constraint_ge ((1i,Y)::(MAP (λ(c,X). (-c,X)) cXs)) 1
+End
+
+Definition cmk_lin_eq_def[simp]:
+  cmk_lin_eq name cXs Y =
+  [
+    (SOME (mk_name name (strlit"ge")), mk_lin_ge cXs Y);
+    (SOME (mk_name name (strlit"le")), mk_lin_le cXs Y)
+  ]
+End
+
+Definition cencode_lin_equal_1_def[simp]:
+  cencode_lin_equal_1 bnd Z cXs Y name =
+  List (
+    MAP (I ## bits_imply bnd [Pos (INL (Ge Z 1))])
+      (cmk_lin_eq name cXs Y))
+End
+
+Definition cencode_lin_equal_2_def[simp]:
+  cencode_lin_equal_2 bnd Z cXs Y name =
+  Append
+    (cencode_lin_equal_1 bnd Z cXs Y name) $
+    Append
+      (cbimply_var bnd (gtv name) (mk_lin_gt cXs Y)) $
+    Append
+      (cbimply_var bnd (ltv name) (mk_lin_lt cXs Y)) $
+    (cat_least_one name
+      [Pos (ltv name); Pos (gtv name); Pos (INL (Ge Z 1))])
+End
+
+Definition encode_lin_equal_def:
+  encode_lin_equal bnd Zr cXs Y name =
+  case Zr of
+    NONE => abstrl (cmk_lin_eq name cXs Y)
+  | SOME (INL Z) =>
+    encode_ge bnd Z 1 ++
+    abstr (cencode_lin_equal_1 bnd Z cXs Y name)
+  | SOME (INR Z) =>
+    encode_ge bnd Z 1 ++
+    abstr (cencode_lin_equal_2 bnd Z cXs Y name)
+End
+
+Theorem eval_icterm_neg[local]:
+  eval_icterm wi ∘ (λ(c,X). (-c,X)) =
+  (λx. -1 * eval_icterm wi x)
+Proof
+  cong_tac NONE>>
+  simp[]>>
+  pairarg_tac>>
+  gs[]>>
+  intLib.ARITH_TAC
+QED
+
+Theorem LAMBDA_eval_icterm[local]:
+  (λx. eval_icterm wi x) = eval_icterm wi
+Proof
+  cong_tac NONE
+QED
+
+Theorem encode_lin_equal_sem_1:
+  valid_assignment bnd wi ∧
+  ALOOKUP cs name = SOME (Linear (Lin reif cmp cXs Y)) ∧
+  reify_sem Zr wi
+    (eval_iclin_term wi cXs = varc wi Y) ⇒
+  EVERY (λx. iconstraint_sem x (wi,reify_avar cs wi))
+    (encode_lin_equal bnd Zr cXs Y name)
+Proof
+  rw[reify_sem_def,encode_lin_equal_def]>>
+  gvs[AllCasePreds(),reify_avar_def,reify_reif_def,reify_flag_def,
+    iconstraint_sem_def,eval_iclin_term_def,eval_icterm_def,
+    iSUM_def,MAP_MAP_o,eval_icterm_neg,iSUM_MAP_lin_const,
+    LAMBDA_eval_icterm]
+  >-intLib.ARITH_TAC
+  >-intLib.ARITH_TAC
+  >-(
+    simp[SF DNF_ss,eval_iclin_term_def,
+      reify_avar_def,reify_reif_def,reify_flag_def]>>
+    intLib.ARITH_TAC)
+QED
+
+Theorem encode_lin_equal_sem_2:
+  valid_assignment bnd wi ∧
+  EVERY (λx. iconstraint_sem x (wi,wb))
+    (encode_lin_equal bnd Zr cXs Y name) ⇒
+  reify_sem Zr wi
+    (eval_iclin_term wi cXs = varc wi Y)
+Proof
+  rw[reify_sem_def,encode_lin_equal_def]>>
+  every_case_tac>>
+  gvs[eval_iclin_term_def,iSUM_def,MAP_MAP_o,eval_icterm_neg,
+    iSUM_MAP_lin_const,LAMBDA_eval_icterm]>>
+  intLib.ARITH_TAC
+QED
+
 (* Linear constraint: Σ ci·Xi cmp Y *)
 Definition encode_lin_def:
   encode_lin bnd Zr cmp Xs Y =
@@ -62,6 +169,42 @@ Proof
 QED
 
 (* Concrete encodings *)
+Definition cencode_lin_equal_def:
+  cencode_lin_equal bnd Zr cXs Y name ec =
+  case Zr of
+    NONE => (List (cmk_lin_eq name cXs Y),ec)
+  | SOME (INL Z) =>
+      let
+        (e,ec') = cencode_ge bnd Z 1 ec
+      in
+        (Append e $ cencode_lin_equal_1 bnd Z cXs Y name, ec')
+  | SOME (INR Z) =>
+      let
+        (e,ec') = cencode_ge bnd Z 1 ec
+      in
+        (Append e $ cencode_lin_equal_2 bnd Z cXs Y name, ec')
+End
+
+Theorem cencode_lin_equal_sem:
+  valid_assignment bnd wi ∧
+  cencode_lin_equal bnd Zr cXs Y name ec = (es, ec') ⇒
+  enc_rel wi es (encode_lin_equal bnd Zr cXs Y name) ec ec'
+Proof
+  rw[cencode_lin_equal_def,encode_lin_equal_def]>>
+  gvs[AllCaseEqs(),UNCURRY_EQ]
+  >-simp[enc_rel_List_refl_mul]
+  >-(
+    irule enc_rel_Append>>
+    irule_at Any enc_rel_encode_ge>>
+    simp[enc_rel_List_refl_mul])
+  >-(
+    irule enc_rel_Append>>
+    irule_at Any enc_rel_encode_ge>>
+    simp[]>>
+    irule enc_rel_abstr_cong>>
+    simp[])
+QED
+
 Definition cencode_linear_constr_def:
   cencode_linear_constr bnd c name ec =
   (List [], ec)
